F*/F* tutorial/Ex10.fst
@@ -1,0 +1,135 @@
+module Ex10
+
+
+open FStar.All
+open FStar.List.Tot
+open FStar.Ref
+
+type file = string
+
+(* Each entry is an element in our access-control list *)
+type entry =
+  | Readable of string
+  | Writable of string
+type db = list entry
+
+(* We define two pure functions that test whether
+   the suitable permission exists in some db *)
+let canWrite db file =
+  Some? (tryFind (function Writable x -> x = file | _ -> false) db)
+
+let canRead db file =
+  Some? (tryFind (function Readable x | Writable x -> x = file) db)
+
+(* The acls reference stores the current access-control list, initially empty *)
+val acls : ref db
+let acls = ST.alloc []
+
+(*
+   Here are two stateful functions which alter the access control list.
+   In reality, these functions may themselves be protected by some
+   further authentication mechanism to ensure that an attacker cannot
+   alter the access control list
+
+   F* infers a fully precise predicate transformer semantics for them.
+*)
+
+
+// Uncomment these types and make them precise enough to pass the test
+// BEGIN: Ex10aExercise
+val grant : e : entry -> ST unit (requires (fun h -> True))
+                                (ensures (fun h x h' -> sel h' acls == (e :: sel h acls)))
+val revoke: e : entry -> ST unit (requires (fun h -> True))
+                                (ensures (fun h x h' -> not (mem e (sel h' acls))))
+// END: Ex10aExercise
+
+
+let grant e = acls := e :: !acls
+
+let revoke e =
+  let db = filter (fun e' -> e <> e') !acls in
+  acls := db
+
+(* Next, we model two primitives that provide access to files *)
+
+(* We use two heap predicates, which will serve as stateful pre-conditions *)
+type canRead_t f h  = canRead  (sel h acls) f == true
+type canWrite_t f h = canWrite (sel h acls) f == true
+
+(* In order to call `read`, you need to prove
+   the `canRead f` permission exists in the input heap *)
+assume val read :  file:string -> ST string
+                                     (requires (canRead_t file))
+                                     (ensures (fun h s h' -> modifies_none h h'))
+
+(* Likewise for `delete` *)
+assume val delete : file:string -> ST unit
+                                     (requires (canWrite_t file))
+                                     (ensures (fun h s h' -> modifies_none h h'))
+
+(* Then, we have a top-level API, which provides protected
+   access to a file by first checking the access control list.
+
+   If the check fails, it raises a fatal exception using `failwith`.
+   As such, it is defined to have effect `All`, which combines
+   both state and exceptions.
+
+   Regardless, the specification proves that `safe_Delete`
+   does not change the heap.
+ *)
+val safe_delete: file -> All unit
+                (requires (fun h -> True))
+                (ensures (fun h x h' -> modifies_none h h'))
+
+
+let safe_delete file =
+  if canWrite !acls file
+  then delete file
+  else failwith "unwritable"
+
+(* Finally, we have a top-level client program *)
+val test_acls: file -> ML unit
+let test_acls f =
+  grant (Readable f);     (* ok *)
+  let _ = read f in       (* ok --- it's in the acl *)
+  //delete f;               (* not ok --- we're only allowed to read it *)
+  safe_delete f;          (* ok, but fails dynamically *)
+  revoke (Readable f);
+  //let _ = read f in       (* not ok any more *)
+  ()
+
+
+
+noeq type point =
+  | Point : x : ref int → y : ref int{addr_of y <>  addr_of x} → point
+
+val new_point: x:int -> y:int -> ST point
+  (requires (fun h -> True))
+  (ensures (fun h0 p h1 ->
+                modifies Set.empty h0 h1
+                /\ fresh (Point?.x p) h0 h1
+                /\ fresh (Point?.y p) h0 h1
+                /\ Heap.sel h1 (Point?.x p) = x
+                /\ Heap.sel h1 (Point?.y p) = y))
+let new_point x y =
+  let x = ST.alloc x in
+  let y = ST.alloc y in
+  Point x y
+
+let shift_x p = Point?.x p := !(Point?.x p) + 1
+
+
+val shift_x_p1: p1:point
+           -> p2:point{   addr_of (Point?.x p2) <> addr_of (Point?.x p1)
+                       /\ addr_of (Point?.y p2) <> addr_of (Point?.x p1) }
+           -> ST unit
+    (requires (fun h -> Heap.contains h (Point?.x p2)
+                    /\  Heap.contains h (Point?.y p2)))
+    (ensures (fun h0 _ h1 -> modifies (only (Point?.x p1)) h0 h1))
+
+let shift_x_p1 p1 p2 =
+    let p2_0 = !(Point?.x p2), !(Point?.y p2)  in //p2 is initially p2_0
+    shift_x p1;
+    let p2_1 = !(Point?.x p2), !(Point?.y p2) in
+    admit(); //fix the precondition and remove the admit
+    assert (p2_0 = p2_1)                         //p2 is unchanged
