F*/F* tutorial/Ex8.fst
@@ -1,0 +1,10 @@
+module Ex8
+
+type vector (a:Type) : nat -> Type =
+   | Nil :  vector a 0
+   | Cons : hd:a -> #n:nat -> tl:vector a n -> vector a (n + 1)
+
+//val reverse_vector: #a:Type -> #n:nat -> vector a n -> Tot (vector a n)
+// is same as
+val reverse_vector: #n:nat -> vector 'a n -> Tot (vector 'a n)
+
